src/Common/CommonPS.v
@@ -1,0 +1,802 @@
+From Coq Require Import FSets.FMapPositive.
+From Coq Require Import FSets.FMapFacts.
+From Coq Require Import List.
+Import ListNotations.
+From Coq Require Import Sorting.Permutation.
+
+From Coq Require Import Setoid.
+From Coq Require Import Relations RelationPairs.
+From Coq Require Import Morphisms.
+
+From Coq Require MSets.MSets.
+From Coq Require Export PArith.
+From Coq Require Import Classes.EquivDec.
+
+From Velus Require Import ClockDefs.
+From Velus Require Import Common.CommonTactics.
+From Velus Require Import Common.CommonList.
+
+(** These modules are used to manipulate identifiers. *)
+
+Module PS := Coq.MSets.MSetPositive.PositiveSet.
+Module PSP := MSetProperties.WPropertiesOn Pos PS.
+Module PSF := MSetFacts.Facts PS.
+Module PSE := MSetEqProperties.WEqPropertiesOn Pos PS.
+Module PSdec := Coq.MSets.MSetDecide.WDecide PS.
+
+Definition ident_eq_dec := Pos.eq_dec.
+Definition ident_eqb := Pos.eqb.
+
+Instance: EqDec ident eq := { equiv_dec := ident_eq_dec }.
+
+Implicit Type i j: ident.
+
+(** ** Properties *)
+
+Definition not_In_empty: forall x : ident, ~(PS.In x PS.empty) := PS.empty_spec.
+
+Ltac not_In_empty :=
+  match goal with H:PS.In _ PS.empty |- _ => now apply not_In_empty in H end.
+
+Lemma not_not_in:
+  forall x A, ~~PS.In x A <-> PS.In x A.
+Proof.
+  split; intro HH.
+  now apply Decidable.not_not in HH; intuition.
+  now apply Decidable.not_not; intuition.
+Qed.
+
+Lemma PS_not_inter:
+  forall s t x,
+    ~PS.In x (PS.inter s t) <-> ~PS.In x s \/ ~PS.In x t.
+Proof.
+  setoid_rewrite PS.inter_spec.
+  split; intro HH.
+  apply Decidable.not_and in HH; auto using PSdec.MSetDecideAuxiliary.dec_In.
+  intuition.
+Qed.
+
+Lemma PS_union_diff_same:
+  forall s t,
+    PS.Equal (PS.union (PS.diff s t) t) (PS.union s t).
+Proof.
+  unfold PS.Equal. setoid_rewrite PS.union_spec.
+  setoid_rewrite PS.diff_spec.
+  split; intro HH. now intuition.
+  destruct HH. now destruct (PSP.In_dec a t); intuition.
+  now intuition.
+Qed.
+
+Lemma PS_not_union:
+  forall s t x,
+    ~PS.In x (PS.union s t) <-> ~PS.In x s /\ ~PS.In x t.
+Proof.
+  setoid_rewrite PS.union_spec.
+  split; intro HH; intuition.
+Qed.
+
+Lemma PS_not_diff:
+  forall s t x,
+    ~PS.In x (PS.diff s t) <-> ~PS.In x s \/ PS.In x (PS.inter s t).
+Proof.
+  setoid_rewrite PS.inter_spec.
+  setoid_rewrite PS.diff_spec.
+  split; intro HH.
+  - apply Decidable.not_and in HH; auto using PSdec.MSetDecideAuxiliary.dec_In.
+    destruct HH as [HH|HH]; auto.
+    apply Decidable.not_not in HH; auto using PSdec.MSetDecideAuxiliary.dec_In.
+    destruct (PSP.In_dec x s); auto.
+  - destruct 1; destruct HH as [|[? ?]]; auto.
+Qed.
+
+Lemma PS_disjoint1:
+  forall s1 s2,
+    PS.Empty (PS.inter s1 s2) ->
+    forall x, PS.In x s1 -> ~PS.In x s2.
+Proof.
+  intros s1 s2 Hdj x Hin1 Hin2.
+  apply (Hdj x). rewrite PS.inter_spec; auto.
+Qed.
+
+Lemma PS_disjoint2:
+  forall s1 s2,
+    PS.Empty (PS.inter s1 s2) ->
+    forall x, PS.In x s2 -> ~PS.In x s1.
+Proof.
+  setoid_rewrite PSP.inter_sym. eauto using PS_disjoint1.
+Qed.
+
+Lemma PS_diff_inter_same:
+  forall A B C,
+    PS.Equal (PS.diff (PS.inter A C) (PS.inter B C))
+             (PS.inter (PS.diff A B) C).
+Proof.
+  intros A B C x. split; intro HH.
+  - apply PS.diff_spec in HH.
+    destruct HH as (HAC & HBC).
+    apply PSP.FM.inter_3; [apply PSP.FM.diff_3|];
+      eauto using PSF.inter_1, PSF.inter_2, PSF.inter_3.
+  - apply PS.inter_spec in HH.
+    destruct HH as (HAB & HC).
+    apply PS.diff_spec in HAB.
+    destruct HAB as (HA & HB).
+    apply PSP.FM.diff_3; [apply PSP.FM.inter_3|];
+      eauto using PSF.inter_1, PSF.inter_2, PSF.inter_3.
+Qed.
+
+Lemma PS_inter_union_dist:
+  forall A B C D,
+    PS.Equal (PS.inter (PS.union A B) (PS.union C D))
+             (PS.union (PS.inter A C)
+                       (PS.union (PS.inter A D)
+                                 (PS.union (PS.inter B C)
+                                           (PS.inter B D)))).
+Proof.
+  intros A B C D.
+  split; intro HH.
+  - rewrite PS.inter_spec in HH.
+    setoid_rewrite PS.union_spec in HH.
+    destruct HH as [[H1|H1] [H2|H2]]; intuition.
+  - repeat setoid_rewrite PS.union_spec in HH.
+    repeat setoid_rewrite PS.inter_spec in HH.
+    destruct HH as [[HH1 HH2]|[[HH1 HH2]|[[HH1 HH2]|[HH1 HH2]]]];
+      intuition.
+Qed.
+
+Lemma PS_inter_inter_same:
+  forall A B C,
+    PS.Equal (PS.inter (PS.inter A C) (PS.inter B C))
+             (PS.inter (PS.inter A B) C).
+Proof.
+  split; intro HH; repeat rewrite PS.inter_spec in *; intuition.
+Qed.
+
+Lemma PS_For_all_Forall:
+  forall P s,
+    PS.For_all P s <-> Forall P (PS.elements s).
+Proof.
+  split; intro HH.
+  - apply Forall_forall.
+    intros x Hin. apply HH.
+    apply PSF.elements_iff; auto.
+  - intros x Hin.
+    rewrite Forall_forall in HH; apply HH.
+    apply PSF.elements_iff, SetoidList.InA_alt in Hin.
+    destruct Hin as (? & ? & ?); subst; auto.
+Qed.
+
+Lemma PS_not_in_diff:
+  forall x s t,
+    ~PS.In x t ->
+    ~PS.In x (PS.diff s t) ->
+    ~PS.In x s.
+Proof.
+  setoid_rewrite PS.diff_spec. intuition.
+Qed.
+
+Lemma PS_For_all_empty:
+  forall P,
+    PS.For_all P PS.empty.
+Proof.
+  setoid_rewrite PS_For_all_Forall.
+  setoid_rewrite PSP.elements_empty. auto.
+Qed.
+
+Lemma PS_In_Forall:
+  forall P S,
+    PS.For_all P S ->
+    forall x, PS.In x S -> P x.
+Proof.
+  intros P S Hfa x Hin.
+  apply PS_For_all_Forall in Hfa.
+  apply PSP.FM.elements_iff in Hin.
+  eapply Forall_forall in Hfa; eauto.
+  apply SetoidList.InA_alt in Hin as (y & Heq & ?).
+  subst; auto.
+Qed.
+
+Lemma PS_For_all_sub:
+  forall P S T,
+    PS.For_all P S ->
+    (forall x, PS.In x T -> PS.In x S) ->
+    PS.For_all P T.
+Proof.
+  intros P S T HP Hsub x HT.
+  apply Hsub in HT.
+  apply PS_In_Forall with (1:=HP) (2:=HT).
+Qed.
+
+Lemma PS_For_all_diff:
+  forall P S T,
+    PS.For_all P S ->
+    PS.For_all P (PS.diff S T).
+Proof.
+  intros P S T HP. apply PS_For_all_sub with (1:=HP).
+  intros x HH; apply PS.diff_spec in HH; intuition.
+Qed.
+
+Lemma PS_For_all_inter:
+  forall P S T,
+    PS.For_all P S ->
+    PS.For_all P (PS.inter S T).
+Proof.
+  intros P S T HP. apply PS_For_all_sub with (1:=HP).
+  intros x HH; apply PS.inter_spec in HH; intuition.
+Qed.
+
+Lemma PS_For_all_union:
+  forall P S T,
+    PS.For_all P S ->
+    PS.For_all P T ->
+    PS.For_all P (PS.union S T).
+Proof.
+  intros P S T HS HT x HH.
+  apply PS.union_spec in HH as [HH|HH]; intuition.
+Qed.
+
+Lemma PS_For_all_impl_In:
+  forall (P Q : PS.elt -> Prop) S,
+    PS.For_all P S ->
+    (forall x, PS.In x S -> P x -> Q x) ->
+    PS.For_all Q S.
+Proof.
+  intros P Q S HP HPQ x HS.
+  apply PS_In_Forall with (2:=HS) in HP; auto.
+Qed.
+
+Instance PS_For_all_Equals_Proper:
+  Proper (pointwise_relation positive iff ==> PS.Equal ==> iff) PS.For_all.
+Proof.
+  intros P Q Hpw S T Heq.
+  split; intros HH x Hx; apply PS_In_Forall with (x:=x) in HH;
+    try apply Hpw; auto.
+  now rewrite Heq. now rewrite Heq in Hx.
+Qed.
+
+Lemma PS_For_all_add:
+  forall P a S,
+    PS.For_all P (PS.add a S) <-> (P a /\ PS.For_all P S).
+Proof.
+  split.
+  - intro HH. split.
+    + apply PS_In_Forall with (1:=HH).
+      now apply PS.add_spec; left.
+    + apply PS_For_all_sub with (1:=HH).
+      intros; apply PS.add_spec; auto.
+  - intros (HPa, HPS) x Hadd.
+    apply PS.add_spec in Hadd as [HH|HH]; subst; auto.
+Qed.
+
+Lemma In_PS_elements:
+  forall x s,
+    In x (PS.elements s) <-> PS.In x s.
+Proof.
+  intros x s. split; intro HH.
+  - now apply (SetoidList.In_InA Pos.eq_equiv), PSF.elements_2 in HH.
+  - cut (exists z, eq x z /\ In z (PS.elements s)).
+    + intros (? & ? & ?); subst; auto.
+    + now apply SetoidList.InA_alt, PSF.elements_1.
+Qed.
+
+Lemma Permutation_elements_add:
+  forall xs x s,
+    Permutation (PS.elements s) xs ->
+    ~PS.In x s ->
+    Permutation (PS.elements (PS.add x s)) (x::xs).
+Proof.
+  intros * Hperm Hnin.
+  setoid_rewrite <- Hperm; clear Hperm.
+  apply NoDup_Permutation.
+  - apply NoDup_NoDupA, PS.elements_spec2w.
+  - constructor; [|now apply NoDup_NoDupA, PS.elements_spec2w].
+    setoid_rewrite PSF.elements_iff in Hnin; auto.
+  - clear. intro z.
+    setoid_rewrite In_PS_elements.
+    setoid_rewrite PS.add_spec.
+    split; intros [HH|HH]; subst; auto.
+    + now constructor.
+    + now constructor 2; apply In_PS_elements.
+    + apply In_PS_elements in HH; auto.
+Qed.
+
+Add Morphism PS.elements
+    with signature PS.Equal ==> @Permutation positive
+        as PS_elements_Equal.
+Proof.
+  intros x y Heq.
+  apply NoDup_Permutation;
+    (try apply NoDup_NoDupA, PS.elements_spec2w).
+  now setoid_rewrite In_PS_elements.
+Qed.
+
+Lemma Permutation_PS_elements_of_list:
+  forall xs,
+    NoDup xs ->
+    Permutation (PS.elements (PSP.of_list xs)) xs.
+Proof.
+  induction xs as [|x xs IH]; auto.
+  rewrite NoDup_cons'. intros (Hxni & Hnd).
+  simpl. specialize (IH Hnd).
+  setoid_rewrite (Permutation_elements_add xs); auto.
+  rewrite PSP.of_list_1.
+  rewrite SetoidList.InA_alt.
+  intros (y & Hxy & Hyin); subst; auto.
+Qed.
+
+Lemma PS_elements_NoDup: forall s,
+    NoDup (PS.elements s).
+Proof.
+  intros s.
+  rewrite NoDup_NoDupA.
+  apply PS.elements_spec2w.
+Qed.
+
+Definition ps_adds (xs: list positive) (s: PS.t) :=
+  fold_left (fun s x => PS.add x s) xs s.
+
+Definition ps_from_list (l: list positive) : PS.t :=
+  ps_adds l PS.empty.
+
+Lemma ps_adds_spec:
+  forall s xs y,
+    PS.In y (ps_adds xs s) <-> In y xs \/ PS.In y s.
+Proof.
+  intros s xs y. revert s.
+  induction xs; intro s; simpl.
+  - intuition.
+  - rewrite IHxs. rewrite PS.add_spec. intuition.
+Qed.
+
+Instance eq_equiv : Equivalence PS.eq.
+Proof. firstorder. Qed.
+
+Instance ps_adds_Proper (xs: list ident) :
+  Proper (PS.eq ==> PS.eq) (ps_adds xs).
+Proof.
+  induction xs as [|x xs IH]; intros S S' Heq; [exact Heq|].
+  assert (PS.eq (PS.add x S) (PS.add x S')) as Heq'
+      by (rewrite Heq; reflexivity).
+  simpl; rewrite Heq'; reflexivity.
+Qed.
+
+Lemma add_ps_from_list_cons:
+  forall xs x,
+    PS.eq (PS.add x (ps_from_list xs))
+          (ps_from_list (x :: xs)).
+Proof.
+  intros; unfold ps_from_list; simpl.
+  generalize PS.empty as S.
+  induction xs as [|y xs IH]; [ reflexivity | ].
+  intro S; simpl; rewrite IH; rewrite PSP.add_add; reflexivity.
+Qed.
+
+Lemma ps_add_eq : forall x1 x2 s,
+    PS.eq (PS.add x1 (PS.add x2 s)) (PS.add x2 (PS.add x1 s)).
+Proof.
+  intros x1 x2 s.
+  split; intros Hin;
+    repeat rewrite PS.add_spec in Hin; destruct Hin as [?|[?|?]]; subst.
+  1,3,4,6: apply PSF.add_2.
+  1,3,5,6: apply PSF.add_1; auto.
+  1,2: apply PSF.add_2; eauto.
+Qed.
+
+Lemma ps_add_adds_eq : forall xs x s,
+    PS.eq (PS.add x (ps_adds xs s)) (ps_adds xs (PS.add x s)).
+Proof.
+  induction xs; intros x s; simpl.
+  - reflexivity.
+  - rewrite IHxs. rewrite ps_add_eq. reflexivity.
+Qed.
+
+Lemma ps_adds_app: forall xs1 xs2 s,
+    PS.eq (ps_adds (xs1 ++ xs2) s)
+          (ps_adds xs1 (ps_adds xs2 s)).
+Proof.
+  induction xs1; intros xs2 s; simpl.
+  - reflexivity.
+  - rewrite IHxs1. rewrite ps_add_adds_eq. reflexivity.
+Qed.
+
+Lemma ps_from_list_In:
+  forall xs x,
+    PS.In x (ps_from_list xs) <-> In x xs.
+Proof.
+  induction xs; simpl.
+  - split; try contradiction; apply not_In_empty.
+  - split; intros * Hin.
+    + rewrite <-IHxs.
+      rewrite <-add_ps_from_list_cons in Hin.
+      apply PSE.MP.Dec.F.add_iff in Hin as []; auto.
+    + rewrite <-IHxs in Hin; rewrite <-add_ps_from_list_cons, PS.add_spec; intuition.
+Qed.
+
+Instance ps_from_list_Permutation:
+  Proper (@Permutation.Permutation ident ==> fun xs xs' => forall x, PS.In x xs -> PS.In x xs')
+         ps_from_list.
+Proof.
+  intros * ?? E ? Hin.
+  apply ps_from_list_In; apply ps_from_list_In in Hin.
+  now rewrite <-E.
+Qed.
+
+Instance ps_from_list_Proper:
+  Proper (@Permutation ident ==> PS.Equal) ps_from_list.
+Proof.
+  intros ? ? Hperm ?.
+  split; intros; rewrite Hperm in *; auto.
+Qed.
+
+Lemma ps_adds_In:
+  forall x xs s,
+    PS.In x (ps_adds xs s) ->
+    ~PS.In x s ->
+    In x xs.
+Proof.
+  induction xs as [|x' xs IH]. now intuition.
+  simpl. intros s Hin Hnin.
+  apply ps_adds_spec in Hin.
+  rewrite PSF.add_iff in Hin.
+  destruct Hin as [|[Hin|Hin]]; intuition.
+Qed.
+
+Lemma Permutation_PS_elements_ps_adds:
+  forall xs S,
+    NoDup xs ->
+    Forall (fun x => ~PS.In x S) xs ->
+    Permutation (PS.elements (ps_adds xs S)) (xs ++ PS.elements S).
+Proof.
+  induction xs as [|x xs IH]; auto.
+  intros S Hnd Hni.
+  apply NoDup_Permutation.
+  - apply NoDup_NoDupA, PS.elements_spec2w.
+  - apply NoDup_app'; auto.
+    apply NoDup_NoDupA, PS.elements_spec2w.
+    apply Forall_impl_In with (2:=Hni).
+    setoid_rewrite In_PS_elements; auto.
+  - apply NoDup_cons' in Hnd as (Hnxs & Hnd).
+    apply Forall_cons2 in Hni as (HnS & Hni).
+    simpl; intro y.
+    setoid_rewrite (IH _ Hnd).
+    + repeat rewrite in_app.
+      repeat rewrite In_PS_elements.
+      rewrite PS.add_spec.
+      split; intros [HH|[HH|HH]]; auto.
+    + apply Forall_impl_In with (2:=Hni).
+      intros z Hzxs Hnzs HzxS.
+      apply PSF.add_3 in HzxS; auto.
+      intro; subst; auto.
+Qed.
+
+Lemma Permutation_PS_elements_ps_adds':
+  forall xs S,
+    NoDup (xs ++ PS.elements S) ->
+    Permutation (PS.elements (ps_adds xs S)) (xs ++ PS.elements S).
+Proof.
+  intros xs S Hnd.
+  rewrite NoDup_app'_iff in Hnd. destruct Hnd as [Hnd1 [_ Hnd2]].
+  eapply Permutation_PS_elements_ps_adds; eauto.
+  eapply Forall_impl; [| eauto].
+  intros a Hnin contra; simpl in *.
+  rewrite In_PS_elements in Hnin. congruence.
+Qed.
+
+Lemma Subset_ps_adds:
+  forall xs S S',
+    PS.Subset S S' ->
+    PS.Subset (ps_adds xs S) (ps_adds xs S').
+Proof.
+  induction xs as [|x xs IH]; auto.
+  intros S S' Hsub. simpl. apply IH.
+  rewrite Hsub. reflexivity.
+Qed.
+
+Definition ps_removes (xs: list positive) (s: PS.t)
+  := fold_left (fun s x => PS.remove x s) xs s.
+
+Lemma ps_removes_spec: forall s xs y,
+    PS.In y (ps_removes xs s) <-> ~In y xs /\ PS.In y s.
+Proof.
+  intros s xs y. revert s.
+  induction xs; intro s; simpl.
+  - intuition.
+  - rewrite IHxs. rewrite PS.remove_spec. intuition.
+Qed.
+
+Lemma ps_removes_app : forall xs1 xs2 s,
+    ps_removes (xs1 ++ xs2) s = ps_removes xs2 (ps_removes xs1 s).
+Proof.
+  induction xs1; intros xs2 s; simpl.
+  - reflexivity.
+  - rewrite IHxs1. reflexivity.
+Qed.
+
+Lemma PS_For_all_ps_adds:
+  forall P xs S,
+    PS.For_all P (ps_adds xs S) <-> (Forall P xs /\ PS.For_all P S).
+Proof.
+  induction xs. now intuition.
+  simpl. setoid_rewrite IHxs.
+  setoid_rewrite Forall_cons2.
+  setoid_rewrite PS_For_all_add.
+  intuition.
+Qed.
+
+Corollary PS_For_all_Forall': forall P xs,
+    PS.For_all P (ps_from_list xs) <-> (Forall P xs).
+Proof.
+  intros P xs.
+  unfold ps_from_list. rewrite PS_For_all_ps_adds.
+  split; intros.
+  - destruct H; auto.
+  - split; auto.
+    apply PS_For_all_empty.
+Qed.
+
+Lemma ps_adds_of_list:
+  forall xs,
+    PS.Equal (ps_adds xs PS.empty) (PSP.of_list xs).
+Proof.
+  intros xs x. rewrite ps_adds_spec, PSP.of_list_1; split.
+  -intros [Hin|Hin]; auto. now apply not_In_empty in Hin.
+  - intro Hin. apply SetoidList.InA_alt in Hin as (y & Hy & Hin); subst; auto.
+Qed.
+
+Corollary ps_from_list_ps_of_list : forall xs,
+    PS.eq (ps_from_list xs) (PSP.of_list xs).
+Proof.
+  intros xs. unfold ps_from_list. apply ps_adds_of_list.
+Qed.
+
+Corollary ps_of_list_In : forall xs x,
+    PS.In x (PSP.of_list xs) <-> In x xs.
+Proof.
+  intros *.
+  rewrite <- ps_from_list_ps_of_list, ps_from_list_In.
+  reflexivity.
+Qed.
+
+Lemma ps_of_list_ps_to_list : forall id xs,
+    In id (PSP.to_list (PSP.of_list xs)) <-> In id xs.
+Proof.
+  intros id xs.
+  specialize (PSP.of_list_2 xs id) as Heq.
+  repeat rewrite InA_alt in Heq.
+  split; intros Hin.
+  - destruct Heq as [[? [? ?]] _]; subst; auto.
+    exists id; auto.
+  - destruct Heq as [_ [? [? ?]]]; subst; auto.
+    exists id; auto.
+Qed.
+
+Lemma ps_of_list_ps_to_list_Perm : forall xs,
+    NoDup xs ->
+    Permutation (PSP.to_list (PSP.of_list xs)) xs.
+Proof.
+  intros xs Hnd; simpl.
+  rewrite <- ps_from_list_ps_of_list.
+  unfold PSP.to_list, ps_from_list.
+  rewrite Permutation_PS_elements_ps_adds';
+    rewrite PSP.elements_empty, app_nil_r; auto.
+Qed.
+
+Inductive DisjointSetList : list PS.t -> Prop :=
+| DJSnil: DisjointSetList []
+| DJScons: forall s ss,
+    DisjointSetList ss ->
+    Forall (fun t => PS.Empty (PS.inter s t)) ss ->
+    DisjointSetList (s :: ss).
+
+Instance DisjointSetList_Proper:
+  Proper (@Permutation.Permutation PS.t ==> iff) DisjointSetList.
+Proof.
+  intros s' s Es.
+  induction Es; split; intro DJ; auto using DisjointSetList;
+    repeat match goal with
+           | H:DisjointSetList (_ :: _) |- _ => inversion_clear DJ
+           | H:_ <-> _ |- _ => destruct H
+           | FA:Forall _ ?xs, H:Permutation ?xs ?ys |- DisjointSetList (_ :: ?ys) =>
+             rewrite H in FA
+           | FA:Forall _ ?ys, H:Permutation ?xs ?ys |- DisjointSetList (_ :: ?xs) =>
+             rewrite <-H in FA
+           | H:Forall _ (_ :: _) |- _ => apply Forall_cons2 in H as (? & ?)
+           | |- DisjointSetList _ => constructor
+           | |- Forall _ (_ :: _) => constructor
+           | H:DisjointSetList (_ :: _) |- _ => inv H
+           | H:PS.Empty (PS.inter ?x ?y) |- PS.Empty (PS.inter ?y ?x) =>
+             now rewrite PSP.inter_sym
+           end; auto using DisjointSetList.
+Qed.
+
+Definition PSUnion (xs : list PS.t) : PS.t :=
+  List.fold_left PS.union xs PS.empty.
+
+Instance fold_left_PS_Proper:
+  Proper ((PS.Equal ==> PS.Equal ==> PS.Equal) ==> eq ==> PS.Equal ==> PS.Equal)
+         (@fold_left PS.t PS.t).
+Proof.
+  intros f g Efg xs' xs Exs S' S ES; subst.
+  revert S S' ES. induction xs; auto.
+  simpl. intros S S' ES. apply IHxs.
+  apply Efg in ES. now apply ES.
+Qed.
+
+Instance PSUnion_Proper:
+  Proper (@Permutation.Permutation PS.t ==> PS.Equal) PSUnion.
+Proof.
+  unfold PSUnion. intros xs ys EE. generalize (PS.empty).
+  induction EE; simpl.
+  - reflexivity.
+  - now setoid_rewrite IHEE.
+  - setoid_rewrite PSP.union_assoc.
+    now setoid_rewrite (PSP.union_sym x).
+  - now setoid_rewrite IHEE1; setoid_rewrite IHEE2.
+Qed.
+
+Instance PSUnion_eqlistA_Proper:
+  Proper (SetoidList.eqlistA PS.Equal ==> PS.Equal) PSUnion.
+Proof.
+  unfold PSUnion. intros xs ys EE. generalize (PS.empty).
+  induction EE; simpl.
+  - reflexivity.
+  - setoid_rewrite IHEE.
+    now take (PS.Equal _ _) and setoid_rewrite it.
+Qed.
+
+Lemma PSUnion_cons:
+  forall T TS, (PSUnion (T :: TS)) === (PS.union T (PSUnion TS)).
+Proof.
+  unfold PSUnion. intros T TS. generalize PS.empty.
+  induction TS; simpl in *. now setoid_rewrite (PSP.union_sym T).
+  intros S.
+  now rewrite <-IHTS, PSP.union_assoc, PSP.union_assoc, (PSP.union_sym T).
+Qed.
+
+Lemma Subset_PSUnion_cons:
+  forall T TS, PS.Subset T (PSUnion (T :: TS)).
+Proof.
+  intros T TS. unfold PSUnion; simpl. revert T.
+  induction TS; simpl; intros T S IST; auto.
+  rewrite <-IHTS. now apply PSF.union_2.
+Qed.
+
+Lemma In_PSUnion:
+  forall T TS,
+    In T TS ->
+    PS.Subset T (PSUnion TS).
+Proof.
+  induction TS. now inversion 1.
+  intro IT. apply in_inv in IT as [IT|IT].
+  - subst. apply Subset_PSUnion_cons.
+  - apply IHTS in IT. rewrite IT, PSUnion_cons.
+    apply PSP.union_subset_2.
+Qed.
+
+Lemma PS_union_empty1:
+  forall s, PS.union PS.empty s === s.
+Proof.
+  intros s x. rewrite PS.union_spec.
+  split; intro HH; auto. destruct HH as [HH|]; auto.
+  inversion HH.
+Qed.
+
+Lemma PS_union_empty2:
+  forall s, PS.union s PS.empty === s.
+Proof.
+  intros s x. rewrite PS.union_spec.
+  split; intro HH; auto. destruct HH as [|HH]; auto.
+  inversion HH.
+Qed.
+
+Lemma PSUnion_cons_empty:
+  forall xs, PSUnion (PS.empty :: xs) === PSUnion xs.
+Proof.
+  setoid_rewrite PSUnion_cons at 1.
+  now setoid_rewrite PS_union_empty1 at 1.
+Qed.
+
+Lemma PSUnion_nil:
+  PSUnion nil = PS.empty.
+Proof.
+  reflexivity.
+Qed.
+
+Lemma PSUnion_app:
+  forall xs ys,
+    PSUnion (PSUnion xs :: ys) === PSUnion (xs ++ ys).
+Proof.
+  induction xs; intro ys; simpl.
+  now rewrite PSUnion_nil, PSUnion_cons_empty.
+  now rewrite PSUnion_cons, PSUnion_cons, PSUnion_cons,
+  <-IHxs, PSUnion_cons, PSP.union_assoc.
+Qed.
+
+Lemma PSUnion_In_app:
+  forall x xs ys,
+    PS.In x (PSUnion (xs ++ ys)) <-> PS.In x (PSUnion xs) \/ PS.In x (PSUnion ys).
+Proof.
+  induction xs; simpl; intro ys.
+  - rewrite PSUnion_nil; split; [intros HH|intros [HH|HH]]; auto.
+    now inv HH.
+  - repeat rewrite PSUnion_cons.
+    now rewrite PS.union_spec, PS.union_spec, IHxs, or_assoc.
+Qed.
+
+Lemma In_In_PSUnion:
+  forall x s ss,
+    PS.In x s ->
+    In s ss ->
+    PS.In x (PSUnion ss).
+Proof.
+  intros x s ss Ix Is.
+  apply in_split in Is as (bl & al & ?); subst.
+  rewrite <-Permutation_middle, PSUnion_cons, PS.union_spec; auto.
+Qed.
+
+Lemma PSUnion_In_In:
+  forall x ss,
+    PS.In x (PSUnion ss) ->
+    exists s, In s ss /\ PS.In x s.
+Proof.
+  induction ss as [|s' ss IH]; intro Ix.
+  now rewrite PSUnion_nil in Ix; inv Ix.
+  rewrite PSUnion_cons, PS.union_spec in Ix; destruct Ix as [Ix|Ix];
+    eauto with datatypes. now firstorder.
+Qed.
+
+Definition In_ps (xs : list positive) (v : PS.t) :=
+  Forall (fun x => PS.In x v) xs.
+
+Lemma In_ps_nil:
+  forall v, In_ps [] v.
+Proof.
+  intro v. apply Forall_nil.
+Qed.
+
+Lemma In_ps_singleton:
+  forall x v,
+    PS.In x v <-> In_ps [x] v.
+Proof.
+  split; intro HH; [|now inv HH].
+  now apply Forall_cons; auto.
+Qed.
+
+Lemma PS_In_In_mem_mem:
+  forall x m n,
+    PS.In x m <-> PS.In x n <-> PS.mem x m = PS.mem x n.
+Proof.
+  intros x m n.
+  destruct (PS.mem x n) eqn:Heq.
+  - rewrite <- PS.mem_spec. intuition.
+  - rewrite <-PSE.MP.Dec.F.not_mem_iff.
+    apply PSE.MP.Dec.F.not_mem_iff in Heq. intuition.
+Qed.
+
+(** Sets and maps of identifiers as efficient list lookups *)
+
+Section Ps_From_Fo_List.
+
+  Context {A : Type} (f: A -> option ident).
+
+  Definition ps_from_fo_list' (xs: list A) (s: PS.t) : PS.t :=
+    fold_left (fun s x=> match f x with
+                      | None => s
+                      | Some i => PS.add i s
+                      end) xs s.
+
+  Definition ps_from_fo_list (xs: list A) : PS.t :=
+    ps_from_fo_list' xs PS.empty.
+
+  Lemma In_ps_from_fo_list':
+    forall x xs s,
+      PS.In x (ps_from_fo_list' xs s) ->
+      PS.In x s \/ In (Some x) (map f xs).
+  Proof.
+    induction xs as [|x' xs IH]; simpl; auto.
+    intros s Hin.
+    destruct (f x'); apply IH in Hin as [Hin|Hin]; auto.
+    destruct (ident_eq_dec i x); subst; auto.
+    rewrite PSF.add_neq_iff in Hin; auto.
+  Qed.
+
+End Ps_From_Fo_List.
